cbor_compare_aux

src/cbor/CBOR.SteelST.Match.fsti
@@ -57,34 +57,26 @@ let raw_data_item_map_match
   (decreases v)
 = SM.seq_list_match c v (raw_data_item_map_entry_match p)
 
-(* `cbor_is_equal_aux` is an auxiliary function intended to compare two CBOR objects
+(* `cbor_compare_aux` is an auxiliary function intended to compare two CBOR objects
    represented by their serialized bytes. It returns an inconclusive result if one of
-   the two is not such an object. The full equality test is implemented in Pulse, see
-   `CBOR.Pulse.cbor_is_equal`
+   the two is not such an object. The full comparison test is implemented in Pulse, see
+   `CBOR.Pulse.cbor_compare`
 *)
 
-noeq [@@no_auto_projectors]
-type cbor_is_equal_aux_t
-= | CborEqual
-  | CborNotEqual
-  | CborCompareFailure
-
 noextract
-let cbor_is_equal_aux_postcond
+let cbor_compare_aux_postcond
   (v1 v2: Cbor.raw_data_item)
-  (res: cbor_is_equal_aux_t)
+  (res: FStar.Int16.t)
 : Tot prop
-= match res with
-  | CborEqual -> v1 == v2
-  | CborNotEqual -> ~ (v1 == v2)
-  | _ -> True
+= let nres = FStar.Int16.v res in
+  (nres = -1 || nres = 0 || nres = 1) ==> nres == Cbor.cbor_compare v1 v2
 
-val cbor_is_equal_aux
+val cbor_compare_aux
   (#p1 #p2: perm)
   (#v1 #v2: Ghost.erased Cbor.raw_data_item)
   (c1 c2: cbor)
-: STT cbor_is_equal_aux_t
+: STT FStar.Int16.t
     (raw_data_item_match p1 c1 v1 `star` raw_data_item_match p2 c2 v2)
     (fun res -> raw_data_item_match p1 c1 v1 `star` raw_data_item_match p2 c2 v2 `star`
-      pure (cbor_is_equal_aux_postcond v1 v2 res)
+      pure (cbor_compare_aux_postcond v1 v2 res)
     )
